\documentclass[20150903-160354-rs2.2-MarksMathNotebook.tex]{subfiles}

\begin{document}
%-=-=-=-=-=-=-=-=-=-=-=-=-=-=-=-=-=-=-=-=-=-=-=-=
%
%	CHAPTER
%
%-=-=-=-=-=-=-=-=-=-=-=-=-=-=-=-=-=-=-=-=-=-=-=-=

\chapter{Derivative Rules}

%-=-=-=-=-=-=-=-=-=-=-=-=-=-=-=-=-=-=-=-=-=-=-=-=
%	SECTION:
%-=-=-=-=-=-=-=-=-=-=-=-=-=-=-=-=-=-=-=-=-=-=-=-=
\section{Derivative of a Monomial Functions}

%-=-=-= EXAMPLE
\begin{example}[id:20141124-153017] \label{20141124-153017}\index{Example!20141124-153017} \hfill \\

Differentiate $f(x)=-3$

\soln

\solnsteps
\begin{align*}
f'(x) &= [-3]' && \text{SPE} \eqref{eq:spe} \\
f'(x) &= 0 && \text{DC} \eqref{eq:dc1}
\end{align*}

\qdepend

\qdependlist

example \ref{20141124-152503}-20141124-152503

\end{example}


%-=-=-= EXAMPLE
\begin{example}[id:20141124-141850] \label{20141124-141850}\index{Example!20141124-141850} \hfill \\

Differentiate $f(x)=x^2$

\soln

\solnsteps
\begin{align*}
f'(x) &= \left[x^2\right]' && \text{SPE} \eqref{eq:spe} \\
f'(x) &= \cRed{2}x^{\cRed{2-1}} && \text{DPo} \eqref{eq:dpo1} \\
f'(x) &= 2x^1 && \text{OOA} \eqref{eq:ooa} \\
f'(x) &= 2x && \text{MId} \eqref{eq:mid2}
\end{align*}

\soln

\lesssteps
\begin{align*}
f'(x) & = 2x && \text{DPo} \eqref{eq:dpo1}
\end{align*}

\qdepend

\qdependlist

example \ref{20141124-141850}-20141124-141850\\
example \ref{20141124-152503}-20141124-152503



\end{example}

%-=-=-=-=-=-=-=-=-=-=-=-=-=-=-=-=-=-=-=-=-=-=-=-=
%	SECTION:
%-=-=-=-=-=-=-=-=-=-=-=-=-=-=-=-=-=-=-=-=-=-=-=-=
\section{Derivative of Polynomial Functions}



%-=-=-= EXAMPLE
\begin{example}[id:20141124-152503] \label{20141124-152503}\index{Example!20141124-152503} \hfill \\

Differentiate $f(x)=x^2-3$

\soln

\solnsteps
\begin{align*}
f(x) &= x^2 + \neg 3 && \text{DOS} \eqref{eq:dos1} \\
f'(x) &= \farg{x^2 + \neg 3}' && \text{SPE} \eqref{eq:spe} \\
f'(x) &= \farg{x^2}' + \farg{\neg 3}' && \text{DS} \eqref{eq:ds1} \\
f'(x) &= \farg{x^2}' + 0 && \text{DC} \eqref{eq:dc1} \\
f'(x) &= \farg{x^2}' && \text{AId} \eqref{eq:aid1} \\
f'(x) &= 2x && \text{DPo} \eqref{eq:dpo1}  \text{\, goto \,}  \ref{20141124-141850}
\end{align*}

\soln

\lesssteps

\begin{align*}
f(x) & = 2x^2 && \text{DPo} \eqref{eq:dpo1} \& \text{DC} \eqref{eq:dpo1}
\end{align*}

\qdepend

\qdependlist

example \ref{20141124-205219}-20141124-205219

\end{example}

%-=-=-= EXAMPLE
\begin{example}[id:20151015-155838] \label{20151015-155838}\index{Example!20151015-155838} \hfill \\
Differentiate $y=x^3+1$

\soln

\solnsteps
\begin{align*}
\farg{y}' &= \farg{x^3+1} && \text{SPE} \eqref{eq:spe} \\
y' &= [x^3]' + [1]' && \text{DS} \eqref{eq:ds1} \\
y' &= 3x^2 + [1]' && \text{DPo} \eqref{eq:dpo1} \\
y' &= 3x^2 + 0 && \text{DC} \eqref{eq:dc1} \\
y' &= 3x^2 && \text{MId} \eqref{eq:mid2} 
\end{align*}

\qdepend

\qdependlist
example \ref{20151015-153507}-20151015-153507

\end{example}

%-=-=-= EXAMPLE
\begin{example}[id:20151011-195002] \label{20151011-195002}\index{Example!20151011-195002} \hfill \\
Differentiate $f(x)=2x^2+3x+7$

\soln

\solnsteps
\begin{align*}
\farg{f'(x)}' &= \farg{2x^2+3x+7}' && \text{SPE} \eqref{eq:spe} \\
f'(x) &= \farg{2x^2}'+\farg{3x}'+\farg{7}' && \text{DS} \eqref{eq:ds1} \\
f'(x) &= 2 \farg{x^2}' + 3\farg{x}' + \farg{7}' && \text{DCM} \eqref{eq:dcm1} \\
f'(x) &= 2 \farg{x^2}' + 3\farg{x}' + 0 && \text{DC} \eqref{eq:dc1} \\
f'(x) &= 2 \farg{x^2}' + 3\farg{x}' && \text{AId} \eqref{eq:aid1} \\
f'(x) &= 2(2x)+3 && \text{DPo} \eqref{eq:dpo1} \\
f'(x) &= 4x + 3 && \text{OOM} \eqref{eq:oom} 
\end{align*}

\qdepend

\qdependlist
example \ref{20151011-154209}-20151011-154209

\end{example}

%-=-=-= EXAMPLE
\begin{example}[id:20141128-151834] \label{20141128-151834}\index{Example!20141128-151834} \hfill \\

Differentiate $f(x)=3x^2-6x+4$

\soln

\solnsteps
\begin{align*}
f(x) &= 3x^2 + \neg 6x + 4 && \text{DOS} \eqref{eq:dos1} \\
f'(x) &= \farg{3x^2 + \neg 6x + 4}' && \text{SPE} \eqref{eq:spe} \\
f'(x) &= \farg{3x^2}' + \farg{6x}' + \farg{4}' && \text{DS} \eqref{eq:ds1} \\
f'(x) &= \farg{3x^2}' + \farg{6x}' + 0 && \text{DC} \eqref{eq:dc1} \\
f'(x) &= \farg{3x^2}' + \farg{6x}' && \text{AId} \eqref{eq:aid1} \\
f'(x) &= 3\farg{x^2}' + 6\farg{x}' && \text{DCM} \eqref{eq:dcm1} \\
f'(x) &= 3 \left(2x \right) + 6 \left(1\right) && \text{DPo} \eqref{eq:dpo1} \\
f'(x) &= 6x+6 && \text{OOM} \eqref{eq:oom}
\end{align*}

\soln
\lesssteps
\begin{align*}
f'(x) & = 6x+6 && \text{DS} \eqref{eq:ds1}
\end{align*}
\end{example}

%-=-=-= EXAMPLE
\begin{example}[id:20141209-144203] \label{20141209-144203}\index{Example!20141209-144203} \hfill \\

Differentiate $f(x)=x^2(2x+4)$

\soln

\solnsteps
\begin{align*}
f'(x)&= \farg{x^2(2x+4)}' && \text{SPE} \eqref{eq:spe} \\
f'(x)&= \farg{x^2}'(2x+4)+x^2\farg{2x+4}' && \text{DPr} \eqref{eq:dpr1} \\
f'(x)&= \farg{x^2}'(2x+4)+x^2\farg{2x}+\farg{4}' && \text{DS} \eqref{eq:ds1} \\
f'(x)&= \farg{x^2}'(2x+4)+x^2 \cdot 2 \farg{x}+\farg{4}' && \text{DCM} \eqref{eq:dcm1} \\
f'(x)&= 2x(2x+4)+ x^2\cdot 2 \cdot 1 + \farg{4}' && \text{DPo} \eqref{eq:dpo1} \\
f'(x)&= 2x(2x+4)+ x^2\cdot 2 \cdot 1 + 0 && \text{DC} \eqref{eq:dc1} \\
f'(x)&= 6x^2+8x && \text{simplify} \text{\, goto \,} \, \ref{20141209-145211}\\
\end{align*}
\end{example}


%-=-=-= EXAMPLE
\begin{example}[id:20141209-142321] \label{20141209-142321}\index{Example!20141209-142321} \hfill \\

Differentiate $f(x)=x^2 \cos(x)$

\soln

\solnsteps
\begin{align*}
f'(x)&= \farg{x^2 \cos(x)}' && \text{SPE} \eqref{eq:spe} \\
f'(x)&= \farg{x^2}' \cos(x) + x^2 \farg{\cos (x)}' && \text{DPr} \eqref{eq:dpr1} \\
f'(x)&= 2x \cos (x) + x^2 \farg{\cos (x)}' && \text{DPo} \eqref{eq:dpo1} \\
f'(x)&= 2x \cos (x) + x^2 (-1 \sin(x)) && \text{DCos} \eqref{eq:dcos1} \\
f'(x)&= 2x \cos (x) - x^2 \sin x && \text{OOM} \eqref{eq:oom}
\end{align*}
\end{example}



%-=-=-= EXAMPLE
\begin{example}[id:20150910-115935] \label{20150910-115935}\index{Example!20150910-115935} \hfill \\

Differentiate $f(x)=\sin(x)\cos(x)$

\soln

\solnsteps
\begin{align*}
f'(x) & = \farg{\sin(x)\cos(x)}' && \text{SPE} \eqref{eq:spe} \\
f'(x) & = \farg{\sin(x)}'\cos(x)+ \sin(x)\farg{\cos(x)}' && \text{DPr} \eqref{eq:dpr1} \\
f'(x) & = \cos (x) \cos (x) + \sin(x)\farg{\cos(x)}' && \text{DSin} \eqref{eq:dsin1} \\
f'(x) &= \cos (x) \cos (x) + \sin(x) (-\sin(x)) && \text{DCos} \eqref{eq:dcos1} \\
f'(x) &= \cos^2(x)-\sin^2(x) && \text{simplify} \text{\, goto \,} \, \ref{} %TODO simplify trigonometric expression
\end{align*}

\end{example}

%-=-=-= EXAMPLE
\begin{example}[id:20141209-151354] \label{20141209-151354}\index{Example!20141209-151354} \hfill \\

Differentiate $f(x)=\sin(x)\sin(x)$

\soln

\solnsteps
\begin{align*}
f'(x) &= \farg{\sin(x)\sin(x)}' && \text{SPE} \eqref{eq:spe} \\
f'(x) &= \farg{\sin(x)}' \sin(x) + \sin (x) \farg{\sin(x)} && \text{DPr} \eqref{eq:dpr1} \\
f'(x) &= \cos(x) \sin(x) + \sin (x) \cos(x) && \text{DSin} \eqref{eq:dsin1} \\
f'(x) &= \cos(x)\sin(x) + \cos(x)\sin(x) && \text{CPM} \eqref{eq:cpm} \\
f'(x) &= 2\cos(x)\sin(x) && \text{OOA} \eqref{eq:ooa} % TODO Simplifying trigonometric expressions
\end{align*}
\end{example}




%-=-=-= EXAMPLE
\begin{example}[id:20141124-203850] \label{20141124-203850}\index{Example!20141124-203850} \hfill \\

Differentiate $y=\ln (3x)$

\soln

\solnsteps

After identifying that $y=\ln (\cRed{3x})$ is a composite function, we let $\cRed{u=3x}$ and thus we get a new function $y=\ln (\cRed{u})$.\\

Using chain rule,
\begin{align*}
\dydx &= \cBlue{\dydu} \cdot \cPurple{\dudx} && \text{DComp} \eqref{eq:dcf2}
\end{align*}

We need to find the factors $\cBlue{\dydu}$ and $\cPurple{\dudx}$.

\begin{alignat*}{2}
		y &= \ln (\cRed{u})				&\quad	 		\cRed{u}		&= 3x \\
	\cBlue{\dydu} &= \dfrac{1}{u}		&\quad 	 \cPurple{\dudx}	 &= 3
\end{alignat*}

\begin{align*}
\dydx &= \cBlue{\dydu} \cdot \cPurple{\dudx} && \text{DComp} \eqref{eq:dcf2} \\
\dydx &= \dfrac{1}{\cRed{u}} \cdot \dudx && \text{DNL} \eqref{eq:dnl1} \\
\dydx &= \dfrac{1}{\cRed{u}} \cdot 3 && \text{DPo} \eqref{eq:dpo1} \\
\dydx &= \dfrac{1}{\cRed{3x}} \cdot 3 \\	% TODO variable subsitution
\dydx &= \dfrac{3}{3x} && \text{OOM} \eqref{eq:oom} \\
\dydx &= \dfrac{1}{x} % TODO reduce fraction
\end{align*}

\qdepend

\qdependlist

example \ref{20141124-205219}-20141124-205219

\end{example}


%-=-=-= EXAMPLE
\begin{example}[id:20141128-160248] \label{20141128-160248}\index{Example!20141128-160248} \hfill \\

Differentiate $y=\ln(3x^2-6x+4)$

\soln

\solnsteps
After identifying that $y=\ln (\cRed{3x^2-6x+4})$ is a composite function, we let \\
$\cRed{u=3x^2-6x+4}$ and thus we get a new function $y=\ln (\cRed{u})$.\\

Using chain rule,
\begin{align*}
\dydx &= \cBlue{\dydu} \cdot \cPurple{\dudx} && \text{DComp} \eqref{eq:dcf2}
\end{align*}

We need to find the factors $\cBlue{\dydu}$ and $\cPurple{\dudx}$.

\begin{alignat*}{3}
		y &= \ln (\cRed{u})				&\quad	 			\cRed{u} 	&= 3x^2-6x+4 	&\quad\\
	\cBlue{\dydu} &= \dfrac{1}{u}		&\quad 	 \cPurple{\dudx}	 &= 6x-6 		&\quad \text{\, goto \,} \, \ref{20141128-151834}
\end{alignat*}

\begin{align*}
\dydx &= \cBlue{\dydu} \cdot \cPurple{\dudx} && \text{DComp} \eqref{eq:dcf2} \\
\dydx &= \dfrac{1}{\cRed{u}} \cdot \dudx && \text{DNL} \eqref{eq:dnl1} \\
\dydx &= \dfrac{1}{\cRed{u}} \cdot (6x-6) && \text{DPo} \eqref{eq:dpo1} \\
\dydx &= \dfrac{1}{\cRed{3x^2-6x+4}} \cdot (6x-6) \\	% TODO variable subsitution
\dydx &= \dfrac{6x-6}{3x^2-6x+4} && \text{OOM} \eqref{eq:oom}
\end{align*}
\end{example}

%-=-=-= EXAMPLE
\begin{example}[id:20141128-155506] \label{20141128-155506}\index{Example!20141128-155506} \hfill \\

Differentiate $y=\ln(\cos x)$

\soln

\solnsteps
After identifying that $y=\ln (\cRed{\cos x})$ is a composite function, we let $\cRed{u=\cos x}$ and thus we get a new function $y=\ln (\cRed{u})$.\\

Using chain rule,
\begin{align*}
\dydx &= \cBlue{\dydu} \cdot \cPurple{\dudx} && \text{DComp} \eqref{eq:dcf2}
\end{align*}

We need to find the factors $\cBlue{\dydu}$ and $\cPurple{\dudx}$.

\begin{alignat*}{2}
		y &= \ln (\cRed{u})				&\quad	 		\cRed{u}		&= \cos x \\
	\cBlue{\dydu} &= \dfrac{1}{u}		&\quad 	 \cPurple{\dudx}	 &= - \sin x
\end{alignat*}

\begin{align*}
\dydx &= \cBlue{\dydu} \cdot \cPurple{\dudx} && \text{DComp} \eqref{eq:dcf2} \\
\dydx &= \dfrac{1}{\cRed{u}} \cdot \dudx && \text{DNL} \eqref{eq:dnl1} \\
\dydx &= \dfrac{1}{\cRed{u}} \cdot - \sin x && \text{DPo} \eqref{eq:dpo1} \\
\dydx &= \dfrac{1}{\cRed{\cos x}} \cdot - \sin x \\	% TODO variable subsitution
\dydx &= \dfrac{-\sin x}{\cos x} && \text{OOM} \eqref{eq:oom} \\
\dydx &= -\tan x % TODO reduce fraction
\end{align*}
\end{example}

%-=-=-= EXAMPLE
\begin{example}[id:20141124-205219] \label{20141124-205219}\index{Example!20141124-205219} \hfill \\

Differentiate $y=\left(x^2-1 \right) \ln(3x)$

\soln

\solnsteps
\begin{align*}
y' &= \farg{x^2-3}' \cdot \ln x + \left(x^2-3\right) \cdot \farg{\ln 3x}' && \text{DPr} \eqref{eq:dpr1} \\
y' &= 2x \cdot \ln x + \left(x^2-3\right) \cdot \farg{\ln 3x}' &&  \text{\, differentiate goto \,} \, \ref{20141124-152503} \\
y' &= 2x \cdot \ln x + \left(x^2-3\right) \cdot \dfrac{1}{x}  && \text{\, differentiate goto \,} \, \ref{20141124-203850}\\
y' &= 2x \cdot \ln x + \dfrac{x^2-3}{x} && \text{OOM} \eqref{eq:oom} \\
y' &= 2x^2 \ln x +\dfrac{x^2-3}{x} && \text{JTC} \eqref{eq:jtc} \\
y' &= \dfrac{2x^2 \ln x + \left(x^2-3\right)}{x} && \text{OOA} \eqref{eq:ooa}
\end{align*}
\end{example}


%-=-=-=-=-=-=-=-=-=-=-=-=-=-=-=-=-=-=-=-=-=-=-=-=
%	SECTION: Derivative of a Quotient
%-=-=-=-=-=-=-=-=-=-=-=-=-=-=-=-=-=-=-=-=-=-=-=-=

\section{Derivative of a Quotient}\label{Derivative of a Quotient}

%-=-=-= EXAMPLE
\begin{example}[id:20151015-165037] \label{20151015-165037}\index{Example!20151015-165037} \hfill \\
Differentiate $y=\dfrac{\sin x}{e^x}$

\soln

\solnsteps
\begin{align*}
\dfrac{\dd \farg{y}}{\dx} &= \dfrac{\dd \farg{\dfrac{\sin x}{e^x}}}{\dx} && \text{SPE} \eqref{eq:spe} \\
\dydx &= \dfrac{\ddx \farg{\sin x} e^x - \sin x \ddx \farg{e^x}}{\farg{e^x}^2} && \text{DQ} \eqref{eq:dq1}\\
\dydx &= \dfrac{\ddx \farg{\sin x} e^x - \sin x \ddx \farg{e^x}}{e^{2x}} && \text{PoPo} \eqref{eq:popo1} \\
\dydx &= \dfrac{\cos x e^x - \sin x \ddx \farg{e^x}}{e^{2x}} && \text{DSin} \eqref{eq:dsin2} \\
\dydx &= \dfrac{\cos x e^x - \sin x e^x}{e^{2x}} && \text{DExp} \eqref{eq:dexp2} \\
\dydx &= \dfrac{e^x (\cos x - \sin x)}{e^{2x}} && \text{DPF} \eqref{eq:dpf2} \\
\dydx &= \dfrac{e^x (\cos x - \sin x)}{e^xe^x} && \text{PrCBPo} \eqref{eq:prcbpo2} \\
\dydx &= \dfrac{\cancel{e^x} (\cos x - \sin x)}{\cancel{e^x}e^x} && \text{MId} \eqref{eq:mid1} \\
\dydx &= \dfrac{\cos x - \sin x}{e^x}
\end{align*}
\end{example}

%-=-=-=-=-=-=-=-=-=-=-=-=-=-=-=-=-=-=-=-=-=-=-=-=
%	SECTION: Derivative of a Rational
%-=-=-=-=-=-=-=-=-=-=-=-=-=-=-=-=-=-=-=-=-=-=-=-=

\section{Derivative of a Rational Function}\label{Derivative of a Rational Function}



%-=-=-= EXAMPLE
\begin{example}[id:20151015-153507] \label{20151015-153507}\index{Example!20151015-153507} \hfill \\
Differentiate $f(x)=\dfrac{x^3+1}{x^2}$

\soln

\solnsteps

Method 1: Derivative of a quotient

\begin{align*}
\farg{f(x)}' &= \farg{\dfrac{x^3+1}{x^2}}' && \text{SPE} \eqref{eq:spe} \\
f'(x) &= \dfrac{\farg{x^3+1}^\prime \left(x^2\right) + \neg 1 \left( \left(x^3+1 \right) \farg{x^2}' \right)}{\farg{x^2}^2} && \text{DQ} \eqref{eq:dq1} \\
f'(x) &= \dfrac{(3x^2)(x^2) \neg 1 \left( \left(x^3+1 \right) \farg{x^2}' \right)}{\farg{x^2}^2} &&  \, \text{\, differentiate goto \,} \, \ref{20151015-155838} \\
f'(x) &= \dfrac{(3x^2)(x^2) \neg 1 \left( \left(x^3+1 \right) (2x) \right)}{\farg{x^2}^2} &&  \, \text{\, differentiate goto \,} \, \ref{20141124-141850} \\
f'(x) &= \dfrac{3x^3-2x^2-2}{x^3} && \text{Simplify \, goto \,} \, \ref{20151015-160832}
\end{align*}
\end{example}

\end{document}

